Cryptonite interpreter code worked out mostly, added example binary to print out protocols

haskell/src/Effects/CryptoniteInterpreter.hs
@@ -28,8 +28,9 @@ import           Unsafe.Coerce
 import           Crypto.Cipher.AES (AES256)
 import           Crypto.Cipher.Types (BlockCipher(..), Cipher(..), makeIV, IV(..))
 import           Crypto.Error (CryptoFailable(..), CryptoError(..))
+import           Crypto.Hash.Algorithms (SHA256(..))
 -- Symmetric Signagures
-import           Crypto.MAC.HMAC (hmac)
+import           Crypto.MAC.HMAC (HMAC(..), hmac)
 -- Asymmetric Operations
 import           Crypto.PubKey.RSA.PKCS15 (decryptSafer, signSafer, encrypt, verify)
 import           Crypto.PubKey.RSA (PublicKey, PrivateKey, generate)
@@ -37,8 +38,9 @@ import           Crypto.PubKey.RSA (PublicKey, PrivateKey, generate)
 import           Crypto.Random (MonadRandom, SystemDRG, withDRG)
 import           Crypto.Random.Types (getRandomBytes)
 
-import           Data.ByteArray (ByteArray)
+import           Data.ByteArray (ByteArray, convert)
 import           Data.ByteString (ByteString)
+import qualified Data.ByteString as BS
 import qualified Data.ByteString.Char8 as C8
 
 import           Data.Function ((&))
@@ -61,58 +63,62 @@ data CryptoKey =
   -- | SymmSigKey ByteString 
   -- | AsymSigKey PublicKey PrivateKey
 
-data StoredCipher =
-  StoredPermission Bool Key ByteString
+data EncMsg =
+  StoredPermission ByteString ByteString
   | StoredContent ByteString
-  | StoredPair StoredCipher StoredCipher
+  | StoredPair EncMsg EncMsg
 
-strToBs :: Show a => a -> ByteString
-strToBs = C8.pack . show
+data StoredCipher =
+  SignedCipher ByteString MsgPayload
+  | EncryptedCipher ByteString EncMsg
 
+-- | Simple utility function to create a ByteString out of anything that can
+-- be converted to a String
+showAsBytes :: Show a => a -> ByteString
+showAsBytes = C8.pack . show
+
+-- | Utility te pull out all data from MsgPayloads in order to build
+-- up a ByteString for digital signature purposes
+msgPayloadAsByteString :: MsgPayload -> ByteString
+msgPayloadAsByteString (R.Coq_message__Permission (kid,tf)) =
+  showAsBytes kid `BS.append` showAsBytes tf
+msgPayloadAsByteString (R.Coq_message__Content i) =
+  showAsBytes i
+msgPayloadAsByteString (R.Coq_message__MsgPair _ _ m1 m2) =
+  msgPayloadAsByteString m1 `BS.append` msgPayloadAsByteString m2
+
+-- | Given an encryption function, convert MsgPayload into a EncMsg
 mkEncCipher :: MonadRandom m =>
-  M.Map Int CryptoKey -> (ByteString -> m ByteString) -> MsgPayload -> m StoredCipher
-mkEncCipher keys enc (R.Coq_message__Permission (kid,tf)) =
-  let k = keys M.! kid
-  in  StoredPermission tf kid <$>
-       case k of
-         SymmKey bs       -> enc bs
-         AsymKey pub priv -> if tf then (enc . strToBs) priv else (enc . strToBs) pub
-
-mkEncCipher _ enc (R.Coq_message__Content i) =
-  StoredContent <$> (enc . C8.pack . show $ i)
-
-mkEncCipher keys enc (R.Coq_message__MsgPair _ _ m1 m2) =
-  do c1 <- mkEncCipher keys enc m1
-     c2 <- mkEncCipher keys enc m2
+  (ByteString -> m ByteString) -> MsgPayload -> m EncMsg
+mkEncCipher enc (R.Coq_message__Permission (kid,tf)) = do
+  kid' <- (enc . showAsBytes) kid
+  tf'  <- (enc . showAsBytes) tf
+  return $ StoredPermission kid' tf'
+mkEncCipher enc (R.Coq_message__Content i) =
+  StoredContent <$> (enc . showAsBytes $ i)
+mkEncCipher enc (R.Coq_message__MsgPair _ _ m1 m2) =
+  do c1 <- mkEncCipher enc m1
+     c2 <- mkEncCipher enc m2
      return $ StoredPair c1 c2
-  
-decryptCipher :: M.Map Int CryptoKey -> (ByteString -> ByteString) -> StoredCipher -> MsgPayload
-decryptCipher keys dec (StoredPermission tf kid bs) =
-  let k = keys M.! kid
-      plain = dec bs
-  in  R.Coq_message__Permission $
-       case k of -- probably want to be handing around keys here, and not ids
-         SymmKey _   -> (kid,True)
-         AsymKey _ _ -> (kid,tf)
 
-decryptCipher _ dec (StoredContent bs) =
-  case C8.readInt (dec bs) of
+-- | Decrypt an EncMsg, given a decryption function
+decryptCipher :: MonadRandom m => (ByteString -> m ByteString) -> EncMsg -> m MsgPayload
+decryptCipher dec (StoredPermission tfenc kidenc) = do
+  tf  <- (read . C8.unpack) <$> dec tfenc
+  kid <- (read . C8.unpack) <$> dec kidenc
+  return $ R.Coq_message__Permission (kid,tf)
+decryptCipher dec (StoredContent bs) = do
+  content <- dec bs
+  case C8.readInt content of
     Nothing    -> error "Decrypting content didn't work"
-    Just (m,_) -> R.Coq_message__Content m
+    Just (m,_) -> return $ R.Coq_message__Content m
+decryptCipher dec (StoredPair c1 c2) = do
+  m1 <- decryptCipher dec c1
+  m2 <- decryptCipher dec c2
+  return $ R.Coq_message__MsgPair Nat Nat m1 m2 -- do I need to track types (that is, little t types?)
 
-decryptCipher keys dec (StoredPair c1 c2) =
-  let m1 = decryptCipher keys dec c1
-      m2 = decryptCipher keys dec c2
-  in  R.Coq_message__MsgPair Nat Nat m1 m2 -- do I need to track types
-
- --  data Coq_message__Coq_message =
- --   Coq_message__Permission RW_message__Coq_access
- -- | Coq_message__Content Prelude.Int
- -- | Coq_message__MsgPair Messages.Coq_type Messages.Coq_type Coq_message__Coq_message Coq_message__Coq_message
-
-
-
-
+-- | Data structure to pass through State monad which handles redirection of
+-- key ids to the actual keys, and cipher ids to the actual ciphers
 data CryptoData = CryptoData {
     ciphers :: M.Map Int StoredCipher
   , keys    :: M.Map Int CryptoKey
@@ -139,6 +145,7 @@ addKey d v cryptoData@CryptoData{..} =
   in
     (k, cryptoData { keys = M.insert k v keys, drg = d })
 
+-- | Helper for BlockCipher encryption
 genRandomIV :: (MonadRandom m, BlockCipher c) => c -> m (IV c)
 genRandomIV c = do
   bs :: ByteString <- getRandomBytes (blockSize c)
@@ -147,27 +154,98 @@ genRandomIV c = do
       Nothing -> error "Couldn't make IV"
       Just iv -> iv
 
-encryptMessage :: MonadRandom m => CryptoKey -> ByteString -> m ByteString
-encryptMessage (AsymKey pub _) msg = do
+-- | Build up an encryption function, given an encryption key.
+-- The key determines which algorith we are using based on whether it
+-- is a symmetric or asymmetric key.  In the future, we probably want
+-- to abstract out the /actual/ algorithms, but that is to be left
+-- for future work.
+encryptFn :: MonadRandom m => CryptoKey -> ByteString -> m ByteString
+encryptFn (AsymKey pub _) msg = do
   eitherMsg <- encrypt pub msg
   return $ case eitherMsg of
              Left e -> error $ "Error asymmetrically encrypting: " ++ show e
              Right m -> m
-encryptMessage (SymmKey k) msg = do
+encryptFn (SymmKey k) msg = do
   iv <- genRandomIV (undefined :: AES256)
   return $ case cipherInit k of
              CryptoFailed e -> error $ "Symmetric encrypt failed: " ++ show e
              CryptoPassed c -> ctrCombine c iv msg
 
-decryptMessage :: MonadRandom m => CryptoKey -> ByteString -> m ByteString
-decryptMessage (AsymKey _ priv) msg = do
+-- | Build up a decryption function, given a decryption key.
+-- The key determines which algorith we are using based on whether it
+-- is a symmetric or asymmetric key.  In the future, we probably want
+-- to abstract out the /actual/ algorithms, but that is to be left
+-- for future work.
+decryptFn :: MonadRandom m => CryptoKey -> ByteString -> m ByteString
+decryptFn (AsymKey _ priv) msg = do
   eitherMsg <- decryptSafer priv msg
   return $ case eitherMsg of
              Left e -> error $ "Error asymmetrically decrypting: " ++ show e
              Right m -> m
-decryptMessage key msg =
-  encryptMessage key msg
+decryptFn key msg =
+  encryptFn key msg
 
+-- | Build up a digital signature function, given a key.
+-- The key determines which algorith we are using based on whether it
+-- is a symmetric or asymmetric key.  In the future, we probably want
+-- to abstract out the /actual/ algorithms, but that is to be left
+-- for future work.
+signatureFn :: MonadRandom m => CryptoKey -> ByteString -> m ByteString
+signatureFn (AsymKey _ priv) msg = do
+  eitherMsg <- signSafer (Just SHA256) priv msg
+  return $ case eitherMsg of
+             Left e -> error $ "Error asymmetrically signing: " ++ show e
+             Right m -> m
+signatureFn (SymmKey k) msg = do
+  let hmacV :: HMAC SHA256 = hmac k msg
+  return ((convert . hmacGetDigest) hmacV)
+
+-- | Encrypt and sign a MsgPayload.  Most of the work is deferred to the helper functions
+-- /signatureFn/ and /encryptFn/.  Handles ordering of encryption vs signing.
+encryptMsgPayload :: MonadRandom m => CryptoKey -> CryptoKey -> MsgPayload -> m StoredCipher
+encryptMsgPayload sigKey encKey msg = do
+  signed <- signMsgPayload sigKey msg
+  case signed of
+    EncryptedCipher _ _ -> error "Cannot happen"
+    SignedCipher sig _ -> do
+      encMsg <- mkEncCipher (encryptFn encKey) msg
+      return $ EncryptedCipher sig encMsg
+
+-- | Encrypt and sign a MsgPayload.  Most of the work is deferred to the helper functions
+-- /signatureFn/ and /decryptFn/.  Handles ordering of encryption vs signing.
+decryptMsgPayload :: MonadRandom m => CryptoKey -> CryptoKey -> StoredCipher -> m MsgPayload
+decryptMsgPayload sigKey encKey (SignedCipher _ _) =
+  error "Already decrypted"
+decryptMsgPayload sigKey encKey (EncryptedCipher sig encMsg) = do
+  msg <- decryptCipher (decryptFn encKey) encMsg
+  ver <- verifyMsgPayload sigKey (SignedCipher sig msg)
+  return msg -- FIXME should probably only return if sig matches
+
+-- | Sign a MsgPayload.  Most of the work is deferred to the helper function
+-- /signatureFn/.  If encryption is to happen, it should happen next.
+signMsgPayload :: MonadRandom m => CryptoKey -> MsgPayload -> m StoredCipher
+signMsgPayload k msg = do
+  sig <- signatureFn k (msgPayloadAsByteString msg)
+  return $ SignedCipher sig msg
+
+-- | Verify the signature on a message.  This function assumes that the
+-- payload has already been decrypted (if it was, in fact encrypted) so
+-- we error out on one branch of the case analysis.  Too bad the types
+-- can't help us out a bit more.  (I guess we could make them more sophisticated,
+-- but we leave that as an exercise to the reader).
+verifyMsgPayload :: MonadRandom m => CryptoKey -> StoredCipher -> m Bool
+verifyMsgPayload (AsymKey pub _) (SignedCipher sig msg) =
+  return $ verify (Just SHA256) pub (msgPayloadAsByteString msg) sig
+verifyMsgPayload (SymmKey k) (SignedCipher sig msg) = do
+  let hmacV :: HMAC SHA256 = hmac k (msgPayloadAsByteString msg)
+  let sig' :: ByteString   = (convert . hmacGetDigest) hmacV
+  return (sig == sig')
+verifyMsgPayload _ _ =
+  error "Unpack your encrypted cipher first"
+
+-- | Here's where the action happens.  Execute each cryptographic command
+-- within our DSL using /cryptonite/ primitives.  All algorithms are currently
+-- hardcoded.  Future work could generalize this.
 runCryptoWithCryptonite :: Member (State CryptoData) r
   => Sem (Crypto : r) a -> Sem r a
 runCryptoWithCryptonite = interpret $ \case
@@ -185,25 +263,37 @@ runCryptoWithCryptonite = interpret $ \case
     let (k,cryptData') = addKey drg' (AsymKey pub priv) cryptData
     _ <- put cryptData'
     (return . unsafeCoerce) (k,True)
-  SignMessage _ _ _ m -> do
+  SignMessage _ kid _ m -> do
     cryptData@CryptoData{..} <- get
-    let (cid,cryptData') = addCipher drg undefined cryptData -- FIXME
-    _ <- put cryptData'
-    (return . unsafeCoerce) (R.SignedCiphertext Nat cid)
-  SignEncryptMessage _ _ kenc _ m -> do
-    cryptData@CryptoData{..} <- get
-    let k = keys M.! kenc
-    let (cipher,drg')    = withDRG drg (mkEncCipher keys (encryptMessage k) m)
+    let k = keys M.! kid
+    let (cipher,drg')    = withDRG drg (signMsgPayload k m)
     let (cid,cryptData') = addCipher drg' cipher cryptData
     _ <- put cryptData'
     (return . unsafeCoerce) (R.SignedCiphertext Nat cid)
-  VerifyMessage _ _ (R.SignedCiphertext _ k) -> do
-    cryptData <- get
-    let m = (ciphers cryptData) M.! k -- use (!) or explicitly case on Maybe?
-    (return . unsafeCoerce) (True, m)
+  SignEncryptMessage _ ksignid kencid _ m -> do
+    cryptData@CryptoData{..} <- get
+    let kenc  = keys M.! kencid
+    let ksign = keys M.! ksignid
+    let (cipher,drg')    = withDRG drg (encryptMsgPayload ksign kenc m)
+    let (cid,cryptData') = addCipher drg' cipher cryptData
+    _ <- put cryptData'
+    (return . unsafeCoerce) (R.SignedCiphertext Nat cid)
+  VerifyMessage _ kid (R.SignedCiphertext _ cid) -> do
+    cryptData@CryptoData{..} <- get
+    let k = keys M.! kid
+    let cipher = ciphers M.! cid -- use (!) or explicitly case on Maybe?
+    let (tf,drg')    = withDRG drg (verifyMsgPayload k cipher)
+    _ <- put cryptData { drg = drg' }
+    (return . unsafeCoerce) $
+      case cipher of
+        SignedCipher _ msg -> (tf, msg)
+        _ -> error "This message is encrypted"
   VerifyMessage _ _ _ -> error "Can only verify ciphertexts"
-  DecryptMessage _ (R.SignedCiphertext _ k) -> do
-    cryptData <- get
-    let m = (ciphers cryptData) M.! k -- use (!) or explicitly case on Maybe?
-    (return . unsafeCoerce) m
+  DecryptMessage _ (R.SignedCiphertext _ cid) -> do
+    cryptData@CryptoData{..} <- get
+    let k = keys M.! 1 -- FIXME
+    let cipher = ciphers M.! cid -- use (!) or explicitly case on Maybe?
+    let (msg,drg')    = withDRG drg (decryptMsgPayload k k cipher)
+    _ <- put cryptData { drg = drg' }
+    (return . unsafeCoerce) msg
   DecryptMessage _ _ -> error "Can only decrypt ciphertexts"
